backends/lean/Aeneas/SimpBoolProp/SimpBoolProp.lean
@@ -11,7 +11,7 @@ open Lean Lean.Meta Lean.Parser.Tactic Lean.Elab.Tactic
 
 attribute [simp_bool_prop_simps]
   reduceIte
-  true_implies false_implies implies_true
+  true_implies false_implies implies_true imp_false
   Bool.and_true Bool.true_and
   Bool.false_or Bool.or_false
   Bool.true_or Bool.or_true
@@ -29,6 +29,8 @@ attribute [simp_bool_prop_simps]
   decide_true decide_false Bool.and_self
   and_self
   iff_false iff_true
+  forall_const
+  exists_false
 
 @[simp_bool_prop_simps]
 theorem not_and_equiv_or_not (a b : Prop) : ¬ (a ∧ b) ↔ ¬ a ∨ ¬ b := by tauto
